spot/GC.SPOT.HeapExpansion.fst
@@ -4215,6 +4215,52 @@ let spot_chunked_forward_one_normal_existing_forwarded_updated_field_edge
   CheneyCorrectness.chunked_forward_one_normal_existing_forwarded_updated_field_edge
     minor cs addr fuel j promoted expected field_addr
 
+let spot_chunked_forward_fields_preserved_forwarded_minor_field_edge
+  (minor: minor_state) (cs: ChunkedCheney.chunked_cheney_state)
+  (parent: U64.t) (idx wosize alloc_fuel: nat)
+  (src expected: obj_addr) (hdr: U64.t) (j: nat)
+  (field_addr: hp_addr) (old: U64.t)
+  : Lemma
+      (requires
+        alloc_fuel > 1 /\
+        GenInv.chunked_major_alloc_shape
+          cs.ccs_major cs.ccs_fp alloc_fuel /\
+        SpecMajorAlloc.major_fl_chain_terminates
+          cs.ccs_major cs.ccs_fp alloc_fuel = true /\
+        GenInv.chunked_chain_objects_blue
+          cs.ccs_major cs.ccs_fp alloc_fuel /\
+        CheneyPreservation.chunked_cheney_forward_fields_split_ready
+          minor cs parent idx wosize alloc_fuel /\
+        Seq.mem src (MH.major_objects cs.ccs_major) /\
+        MH.read_word_in_major cs.ccs_major (hd_address src) == Some hdr /\
+        Obj.getColor hdr <> GC.Lib.Header.Blue /\
+        U64.v (Obj.getTag hdr) < U64.v Obj.no_scan_tag /\
+        j < U64.v (Obj.getWosize hdr) /\
+        U64.v field_addr == U64.v src + j * U64.v mword /\
+        CG.chunked_major_field_slot src j == Some field_addr /\
+        MH.read_word_in_major cs.ccs_major field_addr == Some old /\
+        (let cs' =
+          ChunkedCheney.chunked_cheney_forward_fields
+            minor cs parent idx wosize alloc_fuel in
+         let x = to_minor_offset old in
+         CheneyPreservation.chunked_fwd_targets_above_minor cs'.ccs_fwd /\
+         Seq.mem expected (MH.major_objects cs'.ccs_major) /\
+         is_minor_pointer x /\
+         cs'.ccs_fwd x <> 0UL /\
+         cs'.ccs_fwd x == expected))
+      (ensures
+        (let cs' =
+          ChunkedCheney.chunked_cheney_forward_fields
+            minor cs parent idx wosize alloc_fuel in
+         CG.mem_ce (CG.MajorV src, CG.MajorV expected)
+          (CG.build_chunked_combined_graph
+            (minor_reset minor)
+            (ChunkedUpdate.chunked_update_major_pointers
+              cs'.ccs_major cs'.ccs_fwd))))
+  =
+  CheneyCorrectness.chunked_forward_fields_preserved_forwarded_minor_field_edge
+    minor cs parent idx wosize alloc_fuel src expected hdr j field_addr old
+
 let spot_chunked_cheney_gc_correct_after_preflight_old_major_field_edge
   (minor: minor_state) (major: MH.major_heap) (fp: U64.t)
   (roots: Seq.seq U64.t) (alloc_fuel: nat) (fresh: MH.heap_chunk)
